rename

VST-introduction/ASI_kalloc.v
@@ -8,11 +8,11 @@ doing so in our setup makes ASIs source-program-independent!*)
 Global Open Scope funspec_scope.
 
 Record KallocTokenAPD := {
-  malloc_token': share -> Z -> val -> mpred;
-  malloc_token'_valid_pointer: forall sh sz p, 
-      malloc_token' sh sz p |-- valid_pointer p;
-  malloc_token'_local_facts:  forall sh sz p, 
-      malloc_token' sh sz p |-- !! malloc_compatible sz p;
+  kalloc_token': share -> Z -> val -> mpred;
+  kalloc_token'_valid_pointer: forall sh sz p, 
+      kalloc_token' sh sz p |-- valid_pointer p;
+  kalloc_token'_local_facts:  forall sh sz p, 
+      kalloc_token' sh sz p |-- !! malloc_compatible sz p;
 }.
 
 Record KallocFreeAPD := {
@@ -20,30 +20,30 @@ Record KallocFreeAPD := {
   mem_mgr: globals -> mpred;
 }.
 
-Definition malloc_token {cs:compspecs} M (sh: share) (t: type) (p: val): mpred := 
+Definition kalloc_token {cs:compspecs} M (sh: share) (t: type) (p: val): mpred := 
    !! field_compatible t [] p && 
-   malloc_token' M sh (sizeof t) p.
+   kalloc_token' M sh (sizeof t) p.
 
-Lemma malloc_token_valid_pointer: forall {cs: compspecs} M sh t p, 
-      malloc_token M sh t p |-- valid_pointer p.
-Proof. intros. unfold malloc_token.
- apply andp_left2. apply malloc_token'_valid_pointer.
+Lemma kalloc_token_valid_pointer: forall {cs: compspecs} M sh t p, 
+      kalloc_token M sh t p |-- valid_pointer p.
+Proof. intros. unfold kalloc_token.
+ apply andp_left2. apply kalloc_token'_valid_pointer.
 Qed.
 
-#[export] Hint Resolve malloc_token'_valid_pointer : valid_pointer.
-#[export] Hint Resolve malloc_token_valid_pointer : valid_pointer.
+#[export] Hint Resolve kalloc_token'_valid_pointer : valid_pointer.
+#[export] Hint Resolve kalloc_token_valid_pointer : valid_pointer.
 
-Lemma malloc_token_local_facts:  forall {cs: compspecs} M sh t p,
-      malloc_token M sh t p |-- !! (field_compatible t [] p /\ malloc_compatible (sizeof t) p).
+Lemma kalloc_token_local_facts:  forall {cs: compspecs} M sh t p,
+      kalloc_token M sh t p |-- !! (field_compatible t [] p /\ malloc_compatible (sizeof t) p).
 Proof. intros.
- unfold malloc_token.
+ unfold kalloc_token.
  normalize. rewrite prop_and.
  apply andp_right. apply prop_right; auto.
- apply malloc_token'_local_facts.
+ apply kalloc_token'_local_facts.
 Qed.
 
-#[export] Hint Resolve malloc_token'_local_facts : saturate_local.
-#[export] Hint Resolve malloc_token_local_facts : saturate_local.
+#[export] Hint Resolve kalloc_token'_local_facts : saturate_local.
+#[export] Hint Resolve kalloc_token_local_facts : saturate_local.
 
 Section Kalloc_ASI.
 Variable M: KallocFreeAPD.
@@ -62,7 +62,7 @@ Definition kalloc1_spec :=
        LOCAL (temp ret_temp p)
        SEP ( mem_mgr M gv;
              if eq_dec p nullval then emp
-             else (malloc_token' M Ews n p * memory_block Ews n p)).
+             else (kalloc_token' M Ews n p * memory_block Ews n p)).
 
 Definition kfree1_spec :=
  DECLARE (*_kfree*)kfree1ID
@@ -72,7 +72,7 @@ Definition kfree1_spec :=
        PARAMS (p) GLOBALS (gv)
        SEP (mem_mgr M gv;
             if eq_dec p nullval then emp
-            else (malloc_token' M Ews n p * memory_block Ews n p))
+            else (kalloc_token' M Ews n p * memory_block Ews n p))
     POST [ Tvoid ]
        PROP ()
        LOCAL ()
